src/Ex/Mesi/MesiInvInv1.v
@@ -7,8 +7,6 @@ Require Import Ex.Spec Ex.SpecInds Ex.Template.
 Require Import Ex.Mesi Ex.Mesi.Mesi Ex.Mesi.MesiTopo.
 
 Require Import Ex.Mesi.MesiInv Ex.Mesi.MesiInvInv0.
-Require Import Ex.Mesi.MesiInvEClean.
-        
 
 Set Implicit Arguments.
 
@@ -31,7 +29,7 @@ Definition InvWB (topo: DTree) (st: MState): Prop :=
       ((ObjDirME porq post oidx -> ObjInvWRq oidx (bst_msgs st) ->
         ObjOwned ost) /\
        (ObjDirE porq post oidx -> ObjInvRq oidx (bst_msgs st) ->
-        (ObjClean ost /\ ost#[val] = post#[val]))).
+        ObjClean ost)).
 
 Section InvWB.
   Variable (tr: tree).
